Add functions and tests to PrintTactics.fst

PrintTactics.fst
@@ -29,12 +29,20 @@ let test_fun3 (n : nat) :
   (ensures (fun h1 n' h2 -> n' >= 8)) =
   2 * n
 
+let test_fun4 (n : nat{n >= 2}) :
+  Tot (n':nat{n' >= 8}) =
+  4 * n
+
+let test_fun5 (n : nat{n >= 2}) :
+  Tot (p:(nat & int){let n1, n2 = p in n1 >= 8 /\ n2 >= 2}) =
+  4 * n, 2
+
 let test_lemma1 (n : nat) :
   Lemma (n * n >= 0) = ()
 
 let test_lemma2 (n : nat) :
   Lemma
-  (requires (n >= 4))
+  (requires (n >= 4 /\ True))
   (ensures (2 * n >= 8)) = ()
 
 let predicate_with_a_very_long_name_to_ensure_break_line (n : nat) : Type0 =
@@ -47,7 +55,15 @@ let test_lemma3 (n : nat) :
     predicate_with_a_very_long_name_to_ensure_break_line n))
   (ensures (2 * n >= 8)) = ()
 
-(* Return the qualifier of a term as a string *)
+/// Some constants
+let prims_true_name = "Prims.l_True"
+
+let pure_effect_name = "Prims.PURE"
+let pure_hoare_effect_name = "Prims.Pure"
+let stack_effect_name = "FStar.HyperStack.ST.Stack"
+let st_effect_name = "FStar.HyperStack.ST.ST"
+
+/// Return the qualifier of a term as a string
 val term_qualifier (t : term) : Tac string
 
 let term_qualifier (t : term) : Tac string =
@@ -68,7 +84,7 @@ let term_qualifier (t : term) : Tac string =
   | Tv_AscribedC _ _ _ -> "Tv_AScribedC"
   | _ -> "Tv_Unknown"
 
-(* Return the qualifier of a comp as a string *)
+/// Return the qualifier of a comp as a string
 val comp_qualifier (c : comp) : Tac string
 
 #push-options "--ifuel 1"
@@ -98,11 +114,6 @@ let effect_type_to_string ety =
   | E_ST -> "E_ST"
 #pop-options
 
-let pure_effect_name = "Prims.PURE"
-let pure_hoare_effect_name = "Prims.Pure"
-let stack_effect_name = "FStar.HyperStack.ST.Stack"
-let st_effect_name = "FStar.HyperStack.ST.ST"
-
 val effect_name_to_type (ename : name) : Tot (option effect_type)
 
 let effect_name_to_type (ename : name) : Tot (option effect_type) =
@@ -113,6 +124,68 @@ let effect_name_to_type (ename : name) : Tot (option effect_type) =
   else if ename = st_effect_name then Some E_ST
   else None
 
+/// Refinement type information
+noeq type rtype_info = {
+  raw : typ; // Raw type
+  refin : term; // Refinement predicate
+}
+
+let mk_rtype_info raw refin : rtype_info =
+  Mkrtype_info raw refin
+
+/// Type information
+noeq type type_info = {
+  ty : typ;
+  rty : option rtype_info;
+}
+
+let mk_type_info ty rty : type_info =
+  Mktype_info ty rty
+
+val safe_tc (e:env) (t:term) : Tac (option term)
+
+let safe_tc e t =
+  try Some (tc e t) with | _ -> None
+
+val safe_tcc (e:env) (t:term) : Tac (option comp)
+
+let safe_tcc e t =
+  try Some (tcc e t) with | _ -> None
+
+val get_refin_from_type : typ -> Tac (option term)
+
+let get_refin_from_type t =
+  print ("get_refin_from_type: " ^ term_to_string t);
+  match inspect t with
+  | Tv_Refine bv refin ->
+    print ("Tv_Refine " ^ term_to_string refin);
+    let b : binder = pack_binder bv Q_Explicit in
+    Some (pack (Tv_Abs b refin))
+  | _ -> None
+
+(*let compute_type_refinement
+
+let compute_type_info (e:env) (t:term) : Tac (option type_info) =
+  match safe_tc e t with
+  | None -> None
+  | Some ty ->
+    match inspect ty with
+    | Tv_Refine bv ref ->
+      let b : binder = pack_binder bv Q_Explicit in
+      Some (pack (Tv_Abs b refin))
+  | Tv_Refine : bv:bv -> ref:term -> term_view *)
+
+/// Parameter information
+noeq type param_info = {
+  t : term;
+  qualif : aqualv;
+  ty : option type_info; // The type of the term
+  pty : option type_info; // The type of the expected parameter
+}
+
+let mk_param_info t qualif ty pty : param_info =
+  Mkparam_info t qualif ty pty
+
 /// Effectful term information
 noeq type eterm_info = {
   etype : effect_type;
@@ -120,22 +193,41 @@ noeq type eterm_info = {
   post : option term;
   ret : option typ;
   ret_refin : option term;
+  (* If the term is a function: its head and parameters *)
+  head : term;
+  parameters : list param_info;
   (* ``goal`` is used when the term is the return result of a function:
    * it contains the proof obligation (which is generally a function of
    * the result) *)
   goal : option term;
 }
 
-let mk_eterm_info etype pre post ret ret_refin goal : eterm_info =
-  Mketerm_info etype pre post ret ret_refin goal
+let mk_eterm_info etype pre post ret ret_refin head parameters goal : eterm_info =
+  Mketerm_info etype pre post ret ret_refin head parameters goal
+
+/// Decompose a function application between its body and parameters
+val decompose_application : env -> term -> Tac (term & list param_info)
+
+(* let rec decompose_application_aux (e : env) (t : term) :
+  Tac (term & list param_info) =
+  match inspect t with
+  | Tv_App hd (a, qualif) ->
+    let hd0, params = decompose_application_aux e hd in
+    (* Parameter type *)
+    let ty = safe_tc e a in
+    (* Type expected by the function *)
+    let hd_ty = safe_tc e hd in
+  | _ -> t, []
+Tv_App    : hd:term -> a:argv -> term_view*)
 
 /// Returns the effectful information about a term
 val get_eterm_info : term -> Tac (option eterm_info)
 
 #push-options "--ifuel 1"
 let get_eterm_info (t : term) =
-  (* Retrieve the type of the function *)
   let e = top_env () in
+  (* Decompose the term if it is a function application *)
+  let hd, parameters = t, [] in // TODO
   (* Note that the call to ``tcc`` might fail *)
   try
     begin
@@ -144,32 +236,32 @@ let get_eterm_info (t : term) =
     match cv with
     | C_Total ret_type decr ->
       print ("C_Total: " ^ (term_to_string ret_type));
-      Some (mk_eterm_info E_Total None None (Some ret_type) None None)
+      Some (mk_eterm_info E_Total None None (Some ret_type) None hd parameters None)
     | C_GTotal ret_type decr ->
       print ("C_GTotal: " ^ (term_to_string ret_type));
-      Some (mk_eterm_info E_GTotal None None (Some ret_type) None None)
+      Some (mk_eterm_info E_GTotal None None (Some ret_type) None hd parameters None)
     | C_Lemma pre post patterns ->
       print "C_Lemma:";
       print ("- pre:\n" ^ (term_to_string pre));
       print ("- post:\n" ^ (term_to_string post));
       print ("- patterns:\n" ^ (term_to_string patterns));
-      Some (mk_eterm_info E_Lemma (Some pre) (Some post) None None None)
+      Some (mk_eterm_info E_Lemma (Some pre) (Some post) None None hd parameters None)
     | C_Eff univs eff_name result eff_args ->
       print "C_Eff:";
-      print ("eff_name: " ^ (implode_qn eff_name));
-      print ("result: " ^ (term_to_string result));
-      print "eff_args";
+      print ("- eff_name: " ^ (implode_qn eff_name));
+      print ("- result: " ^ (term_to_string result));
+      print "- eff_args:";
       iter (fun (a, _) -> print ("arg: " ^ (term_to_string a))) eff_args;
       (* Handle the common effects *)
       begin match effect_name_to_type eff_name, eff_args with
       | Some E_PURE, [(pre, _)] ->
-        Some (mk_eterm_info E_PURE (Some pre) None (Some result) None None)
+        Some (mk_eterm_info E_PURE (Some pre) None (Some result) None hd parameters None)
       | Some E_Pure, [(pre, _); (post, _)] ->
-        Some (mk_eterm_info E_Pure (Some pre) (Some post) (Some result) None None)
+        Some (mk_eterm_info E_Pure (Some pre) (Some post) (Some result) None hd parameters None)
       | Some E_Stack, [(pre, _); (post, _)] ->
-        Some (mk_eterm_info E_Stack (Some pre) (Some post) (Some result) None None)
+        Some (mk_eterm_info E_Stack (Some pre) (Some post) (Some result) None hd parameters None)
       | Some E_ST, [(pre, _); (post, _)] ->
-        Some (mk_eterm_info E_ST (Some pre) (Some post) (Some result) None None)
+        Some (mk_eterm_info E_ST (Some pre) (Some post) (Some result) None hd parameters None)
       | _, _ ->
         print ("Unknown or inconsistant effect: " ^ (implode_qn eff_name));
         None
@@ -180,56 +272,76 @@ let get_eterm_info (t : term) =
            (term_to_string t) ^ "'");
     None
 #pop-options
-  
-val simplify_eterm_info : list norm_step -> eterm_info -> Tac eterm_info
+
+/// Check if a proposition is trivial (i.e.: is True)
+val is_trivial_proposition : term -> Tac bool
+
+let is_trivial_proposition t =
+  match inspect t with
+  | Tv_FVar fv ->
+    if implode_qn (inspect_fv fv) = prims_true_name then true else false
+  | _ -> false
+
+/// Simplify the fields of a term and remove the useless ones (i.e.: trivial conditions)
+val simplify_eterm_info : env -> list norm_step -> eterm_info -> Tac eterm_info
 
 #push-options "--ifuel 1"
-let simplify_eterm_info steps info =
-  let e = top_env () in
+let simplify_eterm_info e steps info =
   let opt_norm (x : option term) : Tac (option term) =
-    match x with | Some x' -> Some (norm_term_env e steps x') | None -> None
+    match x with
+    | Some x' -> Some (norm_term_env e steps x')
+    | None -> None
+  in
+  let opt_norm_simplify (x : option term) : Tac (option term) =
+    match opt_norm x with
+    | Some x' -> if is_trivial_proposition x' then None else Some x'
+    | None -> None
   in
   {
     info with
-    pre = opt_norm info.pre;
-    post = opt_norm info.post;
-    ret_refin = opt_norm info.ret_refin;
+    pre = opt_norm_simplify info.pre;
+    post = opt_norm_simplify info.post;
+    ret_refin = opt_norm_simplify info.ret_refin;
+    goal = opt_norm_simplify info.ret_refin;
   }
 #pop-options
 
-val get_type_refin : typ -> Tac (option term)
-
-let get_type_refin t =
-  match inspect t with
-  | Tv_Refine bv refin ->
-    let b : binder = pack_binder bv Q_Explicit in
-    Some (pack (Tv_Abs b refin))
-  | _ -> None
-
 /// Print the effectful information about a term in a format convenient to
 /// use for the emacs commands
-val print_eterm_info : eterm_info -> term -> list term -> Tac unit
+val print_eterm_info : env -> eterm_info -> option string -> term -> list term -> Tac unit
 
+(* TODO: ret_arg: the introduced variables get replaced... *)
 #push-options "--ifuel 1"
-let print_eterm_info info ret_arg post_args =
-    (* Instanciate the post-condition and simplify the info *)
+let print_eterm_info e info ret_arg_name ret_arg post_args =
+    print ("ret_arg: " ^ term_to_string ret_arg);
+    (* Instanciate the post-condition and simplify the information *)
     let spost =
       match info.post with
       | Some post -> Some (mk_e_app post post_args)
       | None -> None
     in
     (* Retrieve the return type refinement, instanciate it and simplify it *)
-    let sret_refin =
+    let sret_refin, e =
       match info.ret with
-      | Some ret ->
-        begin match get_type_refin ret with
-        | Some refin -> Some (mk_e_app ret [ret_arg])
-        | None -> None
+      | Some ret_ty ->
+        (* TODO: get_refin_from_type should have been called before *)
+        begin match get_refin_from_type ret_ty with
+        | Some refin ->
+          let ret_arg, e =
+            match ret_arg_name with
+            | Some name ->
+              let fbv : bv = fresh_bv_named name ret_ty in
+              let b : binder = pack_binder fbv Q_Explicit in
+              pack (Tv_Var fbv), push_binder e b
+            | None -> ret_arg, e
+          in
+          Some (mk_e_app refin [ret_arg]), e
+        | None -> None, e
         end
-      | _ -> None
+      | _ -> None, e
     in
     let info' = { info with post = spost; ret_refin = sret_refin } in
-    let sinfo = simplify_eterm_info [] info' in
+    let sinfo = simplify_eterm_info e [primops; simplify] info' in
     (* Print the information *)
     let print_opt_term name t : Tac unit =
       match t with
@@ -255,45 +367,61 @@ Prims.l_False
 *)
 
 /// The tactic to be called by the emacs commands
-val dprint_eterm : term -> term -> list term -> Tac unit
+val dprint_eterm : term -> option string -> term -> list term -> Tac unit
 
 #push-options "--ifuel 1"
-let dprint_eterm t ret_arg post_args =
+let dprint_eterm t ret_arg_name ret_arg post_args =
   match get_eterm_info t with
   | None ->
     print ("dprint_eterm: could not retrieve effect information from: '" ^
            (term_to_string t) ^ "'")
   | Some info ->
-    print_eterm_info info ret_arg post_args
+    print_eterm_info (top_env ()) info ret_arg_name ret_arg post_args
+#pop-options
 
-let test (x : nat{x >= 4}) : nat =
+let _debug_print_var (name : string) (t : term) : Tac unit =
+  print ("_debug_print_var: " ^ name ^ ": " ^ term_to_string t);
+  begin match safe_tc (top_env ()) t with
+  | Some ty -> print ("type: " ^ term_to_string ty)
+  | _ -> ()
+  end;
+  print ("qualifier: " ^ term_qualifier t);
+  begin match inspect t with
+  | Tv_Var bv ->
+    let b : bv_view = inspect_bv bv in
+    print ("Tv_Var: ppname: " ^ b.bv_ppname ^
+           "; index: " ^ (string_of_int b.bv_index) ^
+           "; sort: " ^ term_to_string b.bv_sort)
+  | _ -> ()
+  end;
+  print "end of _debug_print_var"
+
+let test1 (x : nat{x >= 4}) : nat =
   test_lemma1 x; (**)
+//  run_tactic (fun _ -> dprint_eterm (quote (test_lemma1 x)) (`()) [(`())]);
   (**) test_lemma1 x; (**)
   test_lemma1 (let y = x in y); (**)
   let y = 3 in
   test_lemma1 y;
   test_lemma3 x;
+  let y = test_fun4 x in
+  run_tactic (fun _ -> dprint_eterm (quote (test_fun4 x)) (Some "y") (quote y) [(`())]);
   admit()
-
-(*
-(setq debug-on-error t)
-
-assert(2 * x >= 8);
-
-  //
-  (**) let y = test_fun1 x in (**)  
-  (**) let z = 3 in (**)  (**)  
-  run_tactic (fun _ -> dprint_eterm (quote (test_lemma1 x)) (`()) [(`())]);
-//  run_tactic (fun _ -> dprint_eterm (quote x) (`()) []);
-  admit()
+  let n1, n2 = test_fun5 x in
+//  run_tactic (fun _ -> print ("n1: " ^ term_to_string (quote n1)));
+  run_tactic (fun _ -> _debug_print_var "n1" (quote n1));
+  run_tactic (fun _ -> _debug_print_var "n2" (quote n2));
+  run_tactic (fun _ -> dprint_eterm (quote (test_fun5 x)) None (`(`#(quote n1), `#(quote n2))) [(`())]);
   x
 
 
-(*
-
-
-(global-set-key (kbd "C-M-x") 'eval-region)
-
-(setq debug-on-error t)
-
-*)
+let test2 (x : nat{x >= 4}) : nat =
+  test_lemma1 x; (**)
+  (**) test_lemma1 x; (**)
+  test_lemma1 (let y = x in y); (**)
+  test_lemma2 x;
+  test_lemma2 6;
+  let y = 3 in
+  test_lemma1 y;
+  test_lemma3 x;
+  admit()
